template-coq/theories/utils/MCUtils.v
@@ -1,6 +1,7 @@
 From Coq Require Import Nat ZArith Bool.
 
 Require Export MCPrelude
+        MCReflect
         All_Forall
         MCArith
         MCCompare
